Terminierung Addition

TM/Code/NatTM.v
@@ -1,5 +1,5 @@
-Require Import CodeTM MatchNat.
-Require Import Basic.Mono Basic.Nop Combinators.Combinators.
+Require Import TM.Code.CodeTM TM.Code.MatchNat.
+Require Import TM.Basic.Mono Basic.Nop Combinators.Combinators.
 Require Import TM.LiftMN TM.LiftSigmaTau.
 Require Import TM.Compound.TMTac.
 
@@ -83,9 +83,21 @@ Proof.
   }
 Qed.
 
+Lemma Add_step_Computes_ignoreParam :
+  Add_step ⊨c(12)
+           Computes_Rel (Fin.F1) (Fin.F1) _ _ pred ∩
+           Computes2_Rel (Fin.F1) (Fin.FS Fin.F1) (Fin.FS Fin.F1) _ _ _ add_step__f.
+Proof.
+  eapply RealiseIn_monotone.
+  - eapply Add_step_Computes.
+  - omega.
+  - apply subrel_and2. split.
+    + apply Computes_Rel_ignore_param.
+    + apply Computes2_Rel_ignore_param.
+Qed.
+
 
 Definition Add : { M : mTM _ 2 & states M -> unit } := WHILE Add_step.
-
 
 Lemma add_tail_pred_step (x y : nat) :
   tail_plus (Init.Nat.pred x) (add_step__f x y) = tail_plus x y.
@@ -116,4 +128,90 @@ Proof.
   eapply Computes2_Ext_WRealise.
   - apply plus_tail_plus.
   - apply Add_Sem'.
+Qed.
+
+
+
+(* * Termination *)
+
+Fixpoint step_count (n : nat) : nat :=
+  match n with
+  | O => 12
+  | S n' => 13 + step_count n'
+  end.
+
+Lemma step_count_ge_12 (n : nat) :
+  12 <= step_count n.
+Proof. induction n; cbn; omega. Qed.
+
+
+Lemma step_count_pred_ge_13 (n : nat) :
+  13 + step_count (Init.Nat.pred n) <= step_count n.
+Proof.
+  destruct n; cbn.
+Abort.
+
+
+Section Test.
+  Let t0 := midtape [inl START] (inr false) (map inr [] ++ [inl STOP]).
+  Let t1 := midtape [inl START] (inr true) (map inr [false] ++ [inl STOP]).
+  Let t2 := midtape [inl START] (inr true) (map inr [true; false] ++ [inl STOP]).
+  Let t3 := midtape [inl START] (inr true) (map inr [true; true; false] ++ [inl STOP]).
+  Let t4 := midtape [inl START] (inr true) (map inr [true; true; true; false] ++ [inl STOP]).
+
+  Compute execTM (projT1 Add) (step_count 0) [|t0; t0|].
+  Compute execTM (projT1 Add) (step_count 0) [|t0; t4|].
+  Compute execTM (projT1 Add) (step_count 1) [|t1; t3|].
+  Compute execTM (projT1 Add) (step_count 2) [|t2; t3|].
+  Compute execTM (projT1 Add) (step_count 3) [|t3; t3|].
+  Compute execTM (projT1 Add) (step_count 3) [|t3; t4|].
+  Compute execTM (projT1 Add) (step_count 4) [|t4; t0|].
+End Test.
+
+
+
+
+Lemma Add_terminatesIn :
+  projT1 Add ↓ (fun tin steps => exists x y : nat, tin[@Fin.F1] ≂ x /\ tin[@Fin.FS Fin.F1] ≂ y /\ step_count x = steps).
+Proof.
+  eapply While_terminatesIn.
+  {
+    eapply WRealise_strengthen.
+    - eapply RealiseIn_WRealise. apply Add_step_Computes.
+    - eapply WRealise_R_mTM.
+  }
+  {
+    eapply RealiseIn_terminatesIn. eapply Add_step_Computes.
+  }
+  {
+    eapply functionalOn_intersect. left. eapply functional_functionalOn. eapply R_canonical_functional.
+  }
+  {
+    intros tin ? (m&n&HEncM&HEncN&<-).
+    pose proof (Add_step_Computes tin) as (outc&H1&H2&H3).
+    hnf in H1, H2, H3. specialize (H2 _ HEncM) as (H2&H2'); specialize (H3 _ _ HEncM HEncN) as (H3&H3').
+    exists (ctapes outc), (fst (projT2 Add_step (cstate outc))), (snd (projT2 Add_step (cstate outc))), 12. do 2 split.
+    - hnf. exists outc, 12. split; auto; split; auto. now rewrite <- surjective_pairing.
+    - split.
+      + hnf. intros ? <- % (tape_encodes_injective HEncM). split; auto. now rewrite <- surjective_pairing.
+      + hnf. intros ? ? <- % (tape_encodes_injective HEncM) <- % (tape_encodes_injective HEncN). split; auto.
+        now rewrite <- surjective_pairing.
+    - omega.
+    - destruct (fst _) eqn:E1.
+      +
+        destruct m as [ | m'].
+        {
+          (* m must have been [false]! *)
+          exfalso. cbn in H2, H3, H3'. unfold add_step__p2 in H3'. cbn in H3'.
+          enough (fst (projT2 Add_step (cstate outc)) = false) as L.
+          { enough (true = false) by congruence. now rewrite <- E1, <- L. }
+          unfold finType_CS in *; cbn in *. now rewrite H3'.
+        }
+        {
+          replace (12 + 1) with 13 by reflexivity. eexists. split.
+          * exists m', (add_step__f (S m') n). repeat split. eauto. eauto.
+          * cbn. constructor.
+        }
+      + apply step_count_ge_12.
+  }
 Qed.
